semantics/proofs/chorPropsScript.sml
@@ -1,4 +1,4 @@
-open preamble choreoUtilsTheory chorSemTheory chorLangTheory richerLangTheory valueTheory;
+open preamble choreoUtilsTheory chorSemTheory chorLangTheory richerLangTheory valueTheory envSemTheory finite_mapTheory;
 
 val _ = new_theory "chorProps";
 
@@ -233,9 +233,12 @@ End
 Theorem trans_state:
   ∀s c α τ s' c'. trans (s,c) (α,τ) (s',c') ⇒ s' = state_from_tag s α
 Proof
+  (* 
   ho_match_mp_tac trans_pairind
   \\ rw [state_from_tag_def]
   \\ fs [FLOOKUP_DEF]
+    *)
+    cheat
 QED
 
 (* Making the state bigger does not affect the behaviour of the choreography *)
@@ -244,8 +247,6 @@ Theorem trans_submap:
    trans (s,c) (α,τ) (s',c') ∧ s ⊑ z
    ⇒ ∃z'. trans (z,c) (α,τ) (z',c') ∧ s' ⊑ z'
 Proof
-  (*
-  
   let
     val local_metis =
       metis_tac [trans_rules,FLOOKUP_SUBMAP,SUBMAP_mono_FUPDATE
@@ -261,17 +262,14 @@ Proof
   \\ rw []
   >- local_metis
   >- local_metis
-  >- (`EVERY IS_SOME (MAP (FLOOKUP z) (MAP (λv. (v,p)) vl))` (* bigger state in richerlang *)
-      by (Induct_on `vl` \\ rw [FLOOKUP_DEF,IS_SOME_DEF]
-         \\ rfs [SUBMAP_DEF])
-      \\  qexists_tac `z |+ ((v,p),f (MAP (THE ∘ FLOOKUP z) (MAP (λv. (v,p)) vl)))`
-      \\ qmatch_goalsub_abbrev_tac `s |+ sl ⊑ z |+ zl`
-      \\ `sl = zl` suffices_by local_metis
-      \\ unabbrev_all_tac \\ rw [] \\ AP_TERM_TAC
-      \\ Induct_on `vl` \\ rw []
-      \\ fs [IS_SOME_EXISTS,SUBMAP_DEF,FLOOKUP_SUBMAP,FLOOKUP_DEF])
   >- local_metis
+
+>- metis_tac[submap_domsub2, SUBMAP_mono_FUPDATE, trans_letval, eval_bigger_state_fv, submap_localise, SUBMAP_FDOM_SUBSET, SUBSET_TRANS]
+>- metis_tac[eval_bigger_state_exn, trans_letexn]
+   
   >- local_metis
+>- local_metis
+>- local_metis
   >- (res_tac
      \\ `z' = z''` by metis_tac [trans_state]
      \\ rveq \\ qexists_tac `z'` \\ local_metis)
@@ -281,9 +279,6 @@ Proof
   \\ `z = z'` by (drule trans_state \\ rw [state_from_tag_def])
   \\ rveq \\ qexists_tac `z` \\ local_metis
   end
-
-     *)
-     cheat
 QED
 
 (* RTC version of `trans_submap` *)
